Abandon the use of "ilseg", that is, special-purpose integer-list segments. Instead just use list-segments of "val".  This means that verif1.v needs to mention (lseg (map Vint contents)) from time to time, instead of (ilseg contents), but it is in some ways more honest and straightforward.
Also, avoid the abbrevation "partial_sum" by using subtraction instead.

progs/list.v
@@ -2,6 +2,10 @@ Load loadpath.
 Require Import Coqlib msl.Coqlib2.
 Require Import veric.SeparationLogic.
 Require Import progs.field_mapsto.
+Require Import progs.client_lemmas.
+Require Import Clightdefs.
+Require veric.SequentialClight.
+Import SequentialClight.SeqC.CSL.
 
 Local Open Scope logic.
 
@@ -93,16 +97,16 @@ Definition lseg' (T: type) {ls: listspec T} (sh: share) :=
                  !! (ptr_eq first last) && emp
         end).
 
-Definition lseg (T: type) {ls: listspec T} (sh: share) (contents: list val) (x y: val) : mpred :=
+Definition lseg {T: type} {ls: listspec T} (sh: share) (contents: list val) (x y: val) : mpred :=
    lseg'  T sh (contents, (x,y)).
 
-Lemma lseg_unfold (T: type) {ls: listspec T}: forall sh contents v1 v2,
-    lseg T sh contents v1 v2 = 
+Lemma lseg_unfold {T: type} {ls: listspec T}: forall sh contents v1 v2,
+    lseg sh contents v1 v2 = 
      match contents with
      | h::t => !! (~ ptr_eq v1 v2) && EX tail: val,
                        field_mapsto sh list_struct list_data v1 h 
                       * field_mapsto sh list_struct list_link v1 tail
-                      * |> lseg T sh t tail v2
+                      * |> lseg sh t tail v2
      | nil => !! (ptr_eq v1 v2) && emp
      end.
 Proof.
@@ -119,10 +123,10 @@ Qed.
 Lemma lseg_eq T {ls: listspec T}:
   forall sh l v , 
   typecheck_val v T = true ->
-    lseg T sh l v v = !!(l=nil) && emp.
+    lseg sh l v v = !!(l=nil) && emp.
 Proof.
 intros.
-rewrite (lseg_unfold T sh l v v).
+rewrite (lseg_unfold sh l v v).
 destruct l.
 f_equal. f_equal.
 apply prop_ext; split; intro; auto.
@@ -148,29 +152,29 @@ unfold Int.cmpu.
 rewrite Int.eq_true. auto.
 Qed.
 
-Definition lseg_cons T {ls: listspec T} sh (l: list val) (x z: val) : mpred :=
+Definition lseg_cons {T} {ls: listspec T} sh (l: list val) (x z: val) : mpred :=
         !! (~ ptr_eq x z) && 
        EX h:val, EX r:list val, EX y:val, 
              !!(l=h::r 
                 /\ typecheck_val h list_dtype  = true/\ typecheck_val y T = true) && 
              field_mapsto sh list_struct list_data x h * 
              field_mapsto sh list_struct list_link x y * 
-             |> lseg T sh r y z.
+             |> lseg sh r y z.
 
 
 Lemma lseg_neq:
-  forall T {ls: listspec T} sh l x z , 
+  forall {T} {ls: listspec T} sh l x z , 
   typecheck_val x T = true ->
   typecheck_val z T = true ->
   ptr_neq x z -> 
-    lseg T sh l x z = lseg_cons T sh l x z.
+    lseg sh l x z = lseg_cons sh l x z.
 Proof.
 unfold lseg_cons, ptr_neq; intros.
 rewrite lseg_unfold at 1; auto.
 destruct l.
 apply pred_ext; normalize.
 intros.
-destruct H2; inv H2.
+inv H2.
 apply pred_ext; normalize.
 apply exp_right with v; normalize.
 apply exp_right with l; normalize.
@@ -210,12 +214,10 @@ intros.
 inv H2.
 apply exp_right with y.
 normalize.
-inv H3.
-auto.
 Qed.
 
-Lemma lseg_unroll: forall T {ls: listspec T} sh l x z , 
-    lseg T sh l x z = (!! (ptr_eq x z) && !! (l=nil) && emp) || lseg_cons T sh l x z.
+Lemma lseg_unroll: forall {T} {ls: listspec T} sh l x z , 
+    lseg sh l x z = (!! (ptr_eq x z) && !! (l=nil) && emp) || lseg_cons sh l x z.
 Proof.
 intros.
 rewrite lseg_unfold at 1.
@@ -237,27 +239,20 @@ pattern (field_mapsto sh list_struct list_link x tail) at 1;
  erewrite (field_mapsto_typecheck_val list_struct list_link sh x tail); try reflexivity.
 normalize.
 apply andp_right; auto.
-apply prop_right; split3; auto.
+apply andp_right; apply prop_right.
 rewrite <- (list_unroll_dtype list_struct).
-rewrite <- H0.
-f_equal.
-unfold unroll_composite; simpl.
-rewrite if_true; auto.
-rewrite <- H1.
-f_equal.
-simpl. 
-rewrite if_false by apply list_data_not_link.
-rewrite if_true by auto. rewrite if_true by auto.
-apply list_type_is.
+simpl in H0. rewrite if_true in H0 by auto. apply H0.
+simpl in H1. rewrite if_false in H1 by apply list_data_not_link.
+rewrite if_true in H1 by auto. rewrite if_true in H1 by auto.
+rewrite (@list_type_is _ ls); auto.
 apply orp_left; normalize.
 unfold lseg_cons.
-normalize. intros.
-destruct H0. inv H0.
+normalize. intros. inv H0.
 apply orp_left.
 normalize. inv H0.
 unfold lseg_cons.
 normalize.
-intros. destruct H0. symmetry in H0; inv H0.
+intros. symmetry in H0; inv H0.
 apply exp_right with y.
 normalize.
 Qed.
@@ -280,8 +275,8 @@ Lemma lseg_unroll_nonempty1 {T} {ls: listspec T}:
     typecheck_val p T = true ->
     P |-- field_mapsto sh list_struct list_data v1 h *
              (field_mapsto sh list_struct list_link v1 p *
-               lseg T sh tail p v2) ->
-    P |-- lseg T sh (h::tail) v1 v2.
+               lseg sh tail p v2) ->
+    P |-- lseg sh (h::tail) v1 v2.
 Proof. intros. rewrite lseg_unroll. apply orp_right2. unfold lseg_cons.
   rewrite prop_true_andp by auto.
   apply exp_right with h. apply exp_right with tail. apply exp_right with p.
@@ -316,7 +311,7 @@ Defined.
 Parameters v v' : val.
 Parameters x y : val.
 Parameter whatever : mpred.
-Goal  lseg mylist Share.top (x::y::nil) v v' |-- whatever.
+Goal  lseg Share.top (x::y::nil) v v' |-- whatever.
 rewrite lseg_unfold by auto.
 normalize.
 intros.
@@ -324,3 +319,144 @@ simpl.
 
 Abort.
 End TestCase.
+
+Lemma lseg_nonnull {T: type}{LS: listspec T}:
+  forall sh s v,
+      typed_true T v ->
+     lseg sh s v nullval = lseg_cons sh s v nullval.
+Proof.
+intros. subst. 
+rewrite lseg_unroll.
+apply pred_ext; normalize.
+apply orp_left; auto. normalize.
+unfold typed_true, strict_bool_val,ptr_eq in *.
+destruct v; simpl in *; try contradiction.
+destruct T; simpl in H; try rewrite H0 in H; try discriminate.
+apply orp_right2. auto.
+Qed.
+
+Lemma lift2_lseg_cons {T: type}{LS: listspec T}: 
+ forall sh s p q, lift2 (lseg_cons sh s)  p q =
+    EX hry:(val * list val * val),
+      match hry with (h,r,y) =>
+       !! (s = h::r) &&
+       (local (lift2 ptr_neq p q) &&
+       (lift2 (field_mapsto sh list_struct list_data) p (lift0 h) *
+        lift2 (field_mapsto sh list_struct list_link) p (lift0 y) *
+        |> lift2 (lseg sh r) (lift0 y) q))
+     end.
+Proof.
+ intros.
+ unfold lseg_cons, lift2. extensionality rho. simpl.
+ unfold local, lift1. unfold ptr_neq.
+ apply pred_ext; normalize.
+(* destruct s; symmetry in H0; inv H0. *)
+ apply exp_right with (h, r, y). normalize.
+ destruct h as [[h r] y]. normalize.
+ apply exp_right with h. normalize. apply exp_right with r.
+ normalize. apply exp_right with y. normalize.
+ apply andp_right.
+ erewrite (field_mapsto_typecheck_val); [ | reflexivity].
+  replace (type_of_field
+         (unroll_composite_fields list_structid list_struct
+            (Fcons list_data list_dtype
+               (Fcons (@list_link T LS) (Tcomp_ptr (@list_structid T LS) noattr) Fnil)))
+         (@list_data T LS)) with list_dtype.
+ forget (field_mapsto sh list_struct list_data (p rho) h ) as A.
+ forget (|>lseg sh r y (q rho)) as B.
+ erewrite (field_mapsto_typecheck_val); [ | reflexivity].
+  replace (type_of_field
+         (unroll_composite_fields list_structid list_struct
+            (Fcons list_data list_dtype
+               (Fcons (@list_link T LS) (Tcomp_ptr (@list_structid T LS) noattr) Fnil)))
+         (@list_link T LS)) with T .
+ normalize.
+ simpl.
+ rewrite if_false by apply list_data_not_link. rewrite if_true by auto.
+ rewrite if_true by auto.  apply list_type_is.
+ pose proof (list_unroll_dtype list_struct).
+ simpl. rewrite if_true by auto.
+ symmetry; apply H0.
+ normalize.
+Qed.
+
+Lemma unfold_lseg_cons{T: type}{LS: listspec T}:
+   forall P Q1 Q R e sh s,
+      local Q1 &&
+      PROPx P (LOCALx Q (SEPx (lift2 (lseg sh s) e (lift0 nullval) :: R))) |-- 
+                        local (lift1 (typed_true (tptr list_struct)) e) ->
+      local Q1 && PROPx P (LOCALx Q (SEPx (lift2 (lseg sh s) e (lift0 nullval) :: R))) |--
+     EX hry: val * list val * val,
+      match hry with (h,r,y) => 
+       !! (s=h::r) &&
+      PROPx P (LOCALx Q 
+        (SEPx (lift2 (field_mapsto sh list_struct list_data) e (lift0 h) ::
+                  lift2 (field_mapsto sh list_struct list_link) e (lift0 y) ::
+                  |> lift2 (lseg sh r) (lift0 y) (lift0 nullval) ::
+                  R)))
+        end.
+Proof.
+intros.
+apply derives_trans with
+(local Q1 && PROPx P (LOCALx Q (SEPx (lift2 (lseg_cons sh s) e (lift0 nullval) :: R)))).
+apply derives_trans with
+(local Q1 && local (lift1 (typed_true (tptr list_struct)) e) &&
+ PROPx P (LOCALx Q (SEPx (lift2 (lseg sh s) e (lift0 nullval) :: R)))).
+apply andp_right; auto.
+apply andp_right; auto.
+apply andp_left1; auto.
+apply andp_left2; auto.
+clear H.
+change SEPx with SEPx'.
+intro rho; unfold PROPx,LOCALx,SEPx',local,tc_expr,tc_lvalue,lift2,lift1,lift0; simpl.
+normalize.
+rewrite lseg_nonnull by (rewrite list_type_is; auto).
+auto.
+rewrite lift2_lseg_cons.
+clear.
+change SEPx with SEPx'.
+intro rho; unfold PROPx,LOCALx,SEPx',local,tc_expr,tc_lvalue,lift2,lift1,lift0; simpl.
+normalize.
+apply exp_right with x;
+destruct x as [[h r] y].
+normalize.
+ repeat rewrite sepcon_assoc.
+ auto.
+Qed.
+
+Lemma semax_lseg_nonnull {T: type}{LS: listspec T}:
+  forall Delta P Q sh s e R c Post,
+   PROPx P (LOCALx (tc_environ Delta :: Q)
+            (SEPx (lift2 (lseg sh s) e (lift0 nullval) :: R))) |-- 
+                        local (lift1 (typed_true (tptr list_struct)) e)  ->
+  (forall (h: val) (r: list val) (y: val), s=h::r ->
+    semax Delta 
+        (PROPx P (LOCALx Q 
+        (SEPx (lift2 (field_mapsto sh list_struct list_data) e (lift0 h) ::
+                  lift2 (field_mapsto sh list_struct list_link) e (lift0 y) ::
+                  |> lift2 (lseg sh r) (lift0 y) (lift0 nullval) ::
+                  R)))) c Post) ->
+  semax Delta (PROPx P (LOCALx Q (SEPx (lift2 (lseg sh s) e (lift0 nullval) :: R)))) c Post.
+Proof.
+intros.
+eapply semax_pre;  [apply unfold_lseg_cons | ].
+eapply derives_trans; [ | apply H].
+normalize.
+apply extract_exists_pre; intros [[h r] y].
+apply semax_extract_prop; intro; auto.
+Qed.
+
+
+Lemma lseg_nil_eq {T: type}{LS: listspec T}: 
+    forall sh p q, lseg sh nil p q = !! (ptr_eq p q) && emp.
+Proof. intros.
+ rewrite lseg_unroll.
+ apply pred_ext.
+ apply orp_left. normalize.
+ normalize. unfold lseg_cons. normalize. inv H0.
+ apply orp_right1. normalize.
+Qed.
+Hint Rewrite @lseg_nil_eq : normalize.
+
+Hint Rewrite @lseg_eq : normalize.
+
